Correct LetPair_wp, add notation for pair let and linear load

proofmode.v
@@ -422,7 +422,7 @@ Fixpoint subst_map (vs : stringmap val) (e : expr) : expr :=
   | EVar y =>
      match StringMap.lookup vs y with
      | Some v => EVal v
-     | None => EVar y
+     | None => e
      end
   | ELam y e => ELam y (subst_map (StringMap.delete y vs) e)
   | ERec f y e =>
@@ -446,16 +446,16 @@ Lemma subst_map_empty e :
   subst_map StringMap.empty e = e.
 Proof. induction e; simpl; by f_equal. Qed.
 
-Lemma subst_map_insert x v e env :
-  subst_map (StringMap.insert x v env) e
-  = subst x v (subst_map (StringMap.delete x env) e).
+Lemma subst_map_insert x v vs e :
+  subst_map (StringMap.insert x v vs) e
+  = subst x v (subst_map (StringMap.delete x vs) e).
 Proof.
-  revert env. induction e; intros env; simpl; try (by f_equal).
+  revert vs. induction e; intros vs; simpl; try (by f_equal).
   - (** Case var *)
     rewrite StringMap.lookup_delete, StringMap.lookup_insert.
     destruct (String.eq_dec _ _); simplify_eq.
     + by destruct (String.eq_dec _ _).
-    + destruct (StringMap.lookup env s) eqn:E; simpl; eauto.
+    + destruct (StringMap.lookup vs s) eqn:E; simpl; eauto.
       by destruct (String.eq_dec _ _).
   - (** Case lam *)
     destruct (String.eq_dec _ _); simplify_eq.
@@ -498,7 +498,7 @@ Proof.
 Qed.
 
 (* ########################################################################## *)
-(** Defined language constructions: let, sum, pair let *)
+(** Defined language constructs: let, sum, pair let, linear load *)
 (* ########################################################################## *)
 
 Notation ELet x e1 e2 := (EApp (ELam x e2) e1).
@@ -517,28 +517,17 @@ Definition sum_case :=
 Notation EMatch e x1 e1 x2 e2 :=
   (EApp (EApp (EApp (EVal sum_case) e) (ELam x1 e1)) (ELam x2 e2)).
 
-
 Definition pair_elim :=
   VClosure "x" (ELam "f"
     (EApp (EApp (EVar "f") (EFst (EVar "x"))) (ESnd (EVar "x")))).
+Notation ELetPair x1 x2 e1 e2 :=
+  (EApp (EApp (EVal pair_elim) e1) (ELam x1 (ELam x2 e2))).
 
 Definition lin_load :=
   VClosure "l" (EPair (EVar "l") (ELoad (EVar "l"))).
-
-Notation ELetPair x1 x2 e1 e2 :=
-  (EApp (EApp (EVal pair_elim) e1) (ELam x1 (ELam x2 e2))).
-Notation ELinLoad e :=
-  (EApp (EVal lin_load) e).
+Notation ELinLoad e := (EApp (EVal lin_load) e).
 
 Opaque wp.
-
-Lemma sepEntails_trans' (P Q R : sepProp) :
-  (Q |~ R) ->
-  (P |~ Q) ->
-  P |~ R.
-Proof.
-  intros ??; by eapply sepEntails_trans.
-Qed.
 
 Lemma Let_wp Phi EPhi x v1 e2 e' :
   TCSimpl (subst x v1 e2) e' ->
@@ -581,20 +570,18 @@ Proof.
   iApply Snd_wp. by iApply App_wp.
 Qed.
 
-Lemma LetPair_wp Phi EPhi x1 x2 v1 v2 e1 e :
-  TCSimpl (subst x1 v1 (subst x2 v2 e)) e1 -> 
-  wp e1 Phi EPhi |~
-  wp (ELetPair x1 x2 (EVal (VPair v1 v2)) e1) Phi EPhi.
+Lemma LetPair_wp Phi EPhi x1 x2 v1 v2 e2 e' :
+  TCSimpl (subst x1 v1 (subst x2 v2 e2)) e' ->
+  wp e' Phi EPhi |~ wp (ELetPair x1 x2 (EVal (VPair v1 v2)) e2) Phi EPhi.
 Proof.
   iIntros (<-) "Hwp".
   iApply App_wp. iApply Lam_wp. iApply Lam_wp.
   iApply App_wp. iApply Fst_wp. iApply App_wp.
   destruct (String.eq_dec x2 x1) as [->|?].
   - iApply Lam_wp. iApply Snd_wp. iApply App_wp. 
-    by do 2 rewrite subst_subst_eq.
-  - iApply Lam_wp. iApply Snd_wp. iApply App_wp.
-    rewrite subst_subst_eq. rewrite subst_subst_neq by congruence.
     by rewrite subst_subst_eq.
+  - iApply Lam_wp. iApply Snd_wp. iApply App_wp.
+    by rewrite subst_subst_neq by congruence.
 Qed.
 
 Lemma LinLoad_wp Phi EPhi l v :
@@ -621,7 +608,7 @@ Module language_notation.
   Notation "e1 ;; e2" := (ESeq e1 e2)
     (at level 100, e2 at level 200,
      format "'[' '[hv' '[' e1 ']' ;;  ']' '/' e2 ']'").
-  Notation "! e" := (ELoad e) (at level 9, right associativity, format "! e").
+  Notation "! e" := (ELoad e) (at level 9, right associativity).
   Notation "e1 <- e2" := (EStore e1 e2) (at level 80).
   Notation "'if:' e1 'then' e2 'else' e3" := (EIf e1 e2 e3)
     (at level 200, e1, e2, e3 at level 200).
@@ -666,10 +653,14 @@ Module language_notation.
   Notation "e1 =: e2" := (EOp EqOp e1 e2) (at level 70, no associativity).
   Notation "e1 <=: e2" := (EOp LeOp e1 e2) (at level 70, no associativity).
   Notation "e1 <: e2" := (EOp LtOp e1 e2) (at level 70, no associativity).
+
+  Notation "'let:' ( x1 , x2 ) := e1 'in' e2" := (ELetPair x1 x2 e1 e2)
+    (at level 200, x1, x2 at level 1, e1, e2 at level 200,
+     format "'[' 'let:'  ( x1 , x2 )  :=  '[' e1 ']'  'in'  '/' e2 ']'").
+  Notation "!! e" := (ELinLoad e) (at level 9, right associativity).
 End language_notation.
 
 Module hoare_notation.
-
   Notation "'WP' e {{ v , Q } } {{ w , R } }" :=
     (wp e (fun v => Q) (fun w => R))
     (at level 20, e, Q, R at level 200,
